refinedVST/typing/function.v
@@ -203,14 +203,7 @@ Section function.
       change expr.sizeof with Ctypes.sizeof.
       rewrite Z.add_0_l; split3; first rep_lia; last done.
       apply la_env_cs_sound; auto. }
-    rewrite memory_block_data_at_rec_default_val //.
-    * iFrame.
-      iPureIntro.
-      split3; auto; rewrite /has_layout_val /=.
-      { split; first apply default_value_fits; done. }
-      { eexists; split; first done; by rewrite Forall_forall. }
-    * unfold Ptrofs.max_unsigned, sizeof in *; rep_lia.
-    * apply H1.
+    rewrite memory_block_weaken; by iFrame.
   Qed.
 
   Transparent memory_block.
